FloatSpec/Test/FlocqConformance.lean
@@ -43,7 +43,7 @@ example :
 example :
     valid_binary_payload (prec := 3) (emax := 4)
       (.F754_nan false 4) = false := by
-  simp [valid_binary_payload, FloatSpec.Core.Digits.digits2_pos,
+  simp [valid_binary_payload, valid_binary, FloatSpec.Core.Digits.digits2_pos,
     FloatSpec.Core.Digits.digits2_Pnat,
     FloatSpec.Core.Digits.digits2_Pnat_bitlength_payload,
     FloatSpec.Core.Zaux.Zlt_bool]
@@ -51,7 +51,7 @@ example :
 example :
     valid_binary_payload (prec := 3) (emax := 4)
       (.F754_nan false 3) = true := by
-  simp [valid_binary_payload, FloatSpec.Core.Digits.digits2_pos,
+  simp [valid_binary_payload, valid_binary, FloatSpec.Core.Digits.digits2_pos,
     FloatSpec.Core.Digits.digits2_Pnat,
     FloatSpec.Core.Digits.digits2_Pnat_bitlength_payload,
     FloatSpec.Core.Zaux.Zlt_bool]
